tweaks

messageInvariantPrototypes/twoPhaseCommit/decentralizedMonotonic/distributedSystem.dfy
@@ -39,8 +39,13 @@ module DistributedSystem {
     ghost predicate WF() {
       Host.GroupWFConstants(hosts)
     }
+
     ghost predicate ValidHostId(id: HostId) {
       id < |hosts|
+    }
+
+    ghost predicate ValidParticipantId(id: int) {
+      0 <= id < |hosts|-1
     }
   }
 
@@ -51,6 +56,27 @@ module DistributedSystem {
       && c.WF()
       && Host.GroupWF(c.hosts, hosts)
     }
+
+    ghost function GetCoordinator(c: Constants) : CoordinatorHost.Variables
+      requires WF(c)
+    {
+      Last(hosts).coordinator
+    }
+
+    ghost function GetParticipant(c: Constants, i: int) : ParticipantHost.Variables
+      requires WF(c)
+      requires c.ValidParticipantId(i)
+    {
+      hosts[i].participant
+    }
+
+    ghost function GetParticipantPreference(c: Constants, i: int) : Vote
+      requires c.WF()
+      requires c.ValidParticipantId(i)
+    {
+      c.hosts[i].participant.preference
+    }
+
   }
 
   datatype Variables = Variables(
@@ -80,13 +106,27 @@ module DistributedSystem {
     {
       UtilitiesLibrary.Last(history)
     }
+
+    ghost function Truncate(c: Constants, i: int) : (v : Variables)
+      requires WF(c)
+      requires 0 < i <= |history|
+      ensures v.WF(c)
+      ensures v.Last() == History(i-1)
+    {
+      Variables.Variables(history[..i], network)
+    }
+  } // end datatype Variables
+
+  ghost predicate InitHosts(c: Constants, h: Hosts)
+  {
+    Host.GroupInit(c.hosts, h.hosts)
   }
 
   ghost predicate Init(c: Constants, v: Variables)
   {
     && v.WF(c)
     && |v.history| == 1
-    && Host.GroupInit(c.hosts, v.History(0).hosts)
+    && InitHosts(c, v.History(0))
     && Network.Init(v.network)
   }
 
@@ -100,12 +140,12 @@ module DistributedSystem {
   }
 
   datatype Step =
-    | HostActionStep(hostid: HostId, msgOps: MessageOps)
+    | HostActionStep(actor: HostId, msgOps: MessageOps)
 
   ghost predicate NextStep(c: Constants, h: Hosts, h': Hosts, n: Network.Variables, n': Network.Variables, step: Step)
     requires h.WF(c) && h'.WF(c)
   {
-    && HostAction(c, h, h', step.hostid, step.msgOps)
+    && HostAction(c, h, h', step.actor, step.msgOps)
     && Network.Next(c.network, n, n', step.msgOps)
   }
 
@@ -123,6 +163,87 @@ module DistributedSystem {
       case CoordinatorVariables(coordinator) => coordinator.decision
       case ParticipantVariables(participant) => participant.decision
   }
-}
+
+/***************************************************************************************
+*                                 History properties                                   *
+***************************************************************************************/
+
+  ghost predicate {:opaque} ValidHistory(c: Constants, v: Variables)
+    requires v.WF(c)
+  {
+    && InitHosts(c, v.History(0))
+    && forall i | 
+      && 1 <= i < |v.history|
+    ::
+    Next(c, v.Truncate(c, i), v.Truncate(c, i+1))
+  }
+
+  ghost predicate IsReceiveStepByActor(c: Constants, v: Variables, i:int, actor: int)
+    requires v.WF(c)
+    requires 1 <= i < |v.history|
+    requires Next(c, v.Truncate(c, i), v.Truncate(c, i+1))
+  {
+    var step :| NextStep(c, v.Truncate(c, i).Last(), v.Truncate(c, i+1).Last(), v.network, v.network, step);
+    && step.msgOps.recv.Some?
+    && step.actor == actor
+  }
+
+  lemma InitImpliesValidHistory(c: Constants, v: Variables)
+    requires Init(c, v)
+    ensures ValidHistory(c, v)
+  {
+    reveal_ValidHistory();
+  }
+
+
+  lemma InvNextValidHistory(c: Constants, v: Variables, v': Variables)
+    requires v.WF(c)
+    requires ValidHistory(c, v)
+    requires Next(c, v, v')
+    ensures ValidHistory(c, v')
+  {
+    reveal_ValidHistory();
+    VariableNextProperties(c, v, v');
+    forall i | 1 <= i < |v'.history|
+    ensures Next(c, v'.Truncate(c, i), v'.Truncate(c, i+1))
+    {
+      if i == |v'.history| - 1 {
+        MessageContainmentPreservesNext(c, v, v', v'.Truncate(c, i), v'.Truncate(c, i+1));
+        assert Next(c, v'.Truncate(c, i), v'.Truncate(c, i+1));
+      } else {
+        assert Next(c, v.Truncate(c, i), v.Truncate(c, i+1));
+        assert v.Truncate(c, i).network.sentMsgs <= v'.Truncate(c, i).network.sentMsgs;
+        MessageContainmentPreservesNext(c, v.Truncate(c, i), v.Truncate(c, i+1), v'.Truncate(c, i), v'.Truncate(c, i+1));
+        assert Next(c, v'.Truncate(c, i), v'.Truncate(c, i+1));
+      }
+    }
+  }
+
+  lemma MessageContainmentPreservesNext(c: Constants, v: Variables, v': Variables, s: Variables, s': Variables)
+    requires v.WF(c)
+    requires s.WF(c)
+    requires Next(c, v, v')
+    requires v.history == s.history
+    requires v'.history == s'.history
+    requires v'.network.sentMsgs <= s'.network.sentMsgs
+    requires s.network.sentMsgs == s'.network.sentMsgs
+    ensures Next(c, s, s')
+  {
+    var dsStep :| NextStep(c, v.Last(), v'.Last(), v.network, v'.network, dsStep);
+    assert NextStep(c, s.Last(), s'.Last(), s.network, s'.network, dsStep); // trigger
+  }
+
+  lemma VariableNextProperties(c: Constants, v: Variables, v': Variables)
+    requires v.WF(c)
+    requires Next(c, v, v')
+    ensures 1 < |v'.history|
+    ensures |v.history| == |v'.history| - 1
+    ensures v.Last() == v.History(|v'.history|-2) == v'.History(|v'.history|-2)
+    ensures forall i | 0 <= i < |v'.history|-1 :: v.History(i) == v'.History(i)
+  {
+    assert 0 < |v.history|;
+    assert 1 < |v'.history|;
+  }
+} // end module Distributed System
 
 
